sort vdom before deleting clauses

Weidenbach_Book/IsaSAT_Arena.thy
@@ -1396,7 +1396,7 @@ lemma arena_lifting:
     \<open>arena_length arena i \<ge> 2\<close> and
     \<open>arena_status arena i = LEARNED \<longleftrightarrow> \<not>irred N i\<close> and
     \<open>arena_status arena i = IRRED \<longleftrightarrow> irred N i\<close> and
-    \<open>arena_status arena i \<noteq> DELETED\<close> 
+    \<open>arena_status arena i \<noteq> DELETED\<close>
 proof -
   have
     dom: \<open>\<And>i. i\<in>#dom_m N \<Longrightarrow>
@@ -1486,10 +1486,10 @@ proof -
     \<open>N \<propto> i ! 0 = arena_lit arena i\<close> and
     \<open>is_Lit (arena ! i)\<close>
     using is_lit[of 0] ge2 by fastforce+
-  show 
+  show
     \<open>arena_status arena i = LEARNED \<longleftrightarrow> \<not>irred N i \<close>and
     \<open>arena_status arena i = IRRED \<longleftrightarrow> irred N i\<close> and
-    \<open>arena_status arena i \<noteq> DELETED\<close> 
+    \<open>arena_status arena i \<noteq> DELETED\<close>
     using learned init unfolding arena_status_def
     by (auto simp: arena_status_def)
 qed
@@ -2399,6 +2399,78 @@ lemma mark_garbage_hnr[sepref_fr_rules]:
   using mark_garbage_code.refine[FCOMP isa_mark_garbage]
   unfolding hr_comp_assoc[symmetric] list_rel_compp status_assn_alt_def uncurry_def
   by (auto simp add: arl_assn_comp update_lbd_pre_def)
+
+
+paragraph \<open>Activity\<close>
+definition arena_act_pre where
+  \<open>arena_act_pre = arena_is_valid_clause_idx\<close>
+
+definition isa_arena_act :: \<open>uint32 list \<Rightarrow> nat \<Rightarrow> uint32 nres\<close> where
+  \<open>isa_arena_act arena C = do {
+      ASSERT(C - ACTIVITY_SHIFT < length arena \<and> C \<ge> ACTIVITY_SHIFT);
+      RETURN (arena ! (C - ACTIVITY_SHIFT))
+  }\<close>
+
+lemma arena_act_conv:
+  assumes
+    valid: \<open>valid_arena arena N x\<close> and
+    j: \<open>j \<in># dom_m N\<close> and
+    a: \<open>(a, arena) \<in> \<langle>uint32_nat_rel O arena_el_rel\<rangle>list_rel\<close>
+  shows
+    \<open>j - ACTIVITY_SHIFT < length arena\<close> (is ?le) and
+    \<open>ACTIVITY_SHIFT \<le> j\<close> (is ?ge) and
+    \<open>(a ! (j - ACTIVITY_SHIFT),
+        xarena_act (arena ! (j - ACTIVITY_SHIFT)))
+       \<in> uint32_nat_rel\<close>
+proof -
+  have j_le: \<open>j < length arena\<close> and
+    length: \<open>length (N \<propto> j) = arena_length arena j\<close> and
+    k1:\<open>\<And>k. k < length (N \<propto> j) \<Longrightarrow> N \<propto> j ! k = arena_lit arena (j + k)\<close> and
+    k2:\<open>\<And>k. k < length (N \<propto> j) \<Longrightarrow> is_Lit (arena ! (j+k))\<close> and
+    le: \<open>j + length (N \<propto> j) \<le> length arena\<close>  and
+    j_ge: \<open>header_size (N \<propto> j) \<le> j\<close> and
+    lbd: \<open>is_Act (arena ! (j - ACTIVITY_SHIFT))\<close>
+    using arena_lifting[OF valid j] by auto
+  show le': ?le
+     using le j_ge unfolding length[symmetric] header_size_def
+     by (auto split: if_splits simp: ACTIVITY_SHIFT_def)
+  show ?ge
+    using j_ge by (auto simp: SHIFTS_def header_size_def split: if_splits)
+  have
+    \<open>(a ! (j - ACTIVITY_SHIFT),
+         (arena ! (j - ACTIVITY_SHIFT)))
+       \<in> uint32_nat_rel O arena_el_rel\<close>
+    by (rule param_nth[OF _ _ a]) (use j_le in auto)
+  then show \<open>(a ! (j - ACTIVITY_SHIFT),
+        xarena_act (arena ! (j - ACTIVITY_SHIFT)))
+       \<in> uint32_nat_rel\<close>
+    using lbd by (cases \<open>arena ! (j - ACTIVITY_SHIFT)\<close>) (auto simp: arena_el_rel_def)
+qed
+
+lemma isa_arena_act_arena_act:
+  \<open>(uncurry isa_arena_act, uncurry (RETURN oo arena_act)) \<in>
+    [uncurry arena_act_pre]\<^sub>f
+     \<langle>uint32_nat_rel O arena_el_rel\<rangle>list_rel \<times>\<^sub>f nat_rel \<rightarrow>
+    \<langle>uint32_nat_rel\<rangle>nres_rel\<close>
+  by (intro frefI nres_relI)
+    (auto simp: isa_arena_act_def arena_act_def arena_get_lbd_conv
+      arena_act_pre_def arena_is_valid_clause_idx_def
+      list_rel_imp_same_length arena_act_conv
+      intro!: ASSERT_leI)
+
+sepref_definition isa_arena_act_code
+  is \<open>uncurry isa_arena_act\<close>
+  :: \<open>(arl_assn uint32_assn)\<^sup>k *\<^sub>a nat_assn\<^sup>k \<rightarrow>\<^sub>a uint32_assn\<close>
+  unfolding isa_arena_act_def ACTIVITY_SHIFT_def
+  by sepref
+
+lemma isa_arena_act_code[sepref_fr_rules]:
+  \<open>(uncurry isa_arena_act_code, uncurry (RETURN \<circ>\<circ> arena_act))
+     \<in> [uncurry arena_act_pre]\<^sub>a arena_assn\<^sup>k *\<^sub>a nat_assn\<^sup>k \<rightarrow> uint32_nat_assn\<close>
+  using isa_arena_act_code.refine[FCOMP isa_arena_act_arena_act]
+  unfolding hr_comp_assoc[symmetric] list_rel_compp status_assn_alt_def uncurry_def
+  by (auto simp add: arl_assn_comp update_lbd_pre_def)
+
 
 
 end
